Add stronger properties to Var iterator and foldmap

Valaig/Aig/Iter.lean
@@ -47,10 +47,10 @@ instance instIterator : Std.Iterator (GenericIter mk size valid) m α where
       .done (by grind)
 
 attribute [local grind =] Std.IterM.Step.toPure_yield Std.IterM.Step.toPure_skip Std.IterM.Step.toPure_done
-attribute [local grind unfold] Std.PlausibleIterStep.yield Std.PlausibleIterStep.skip Std.PlausibleIterStep.done
+attribute [local grind] Std.PlausibleIterStep.yield Std.PlausibleIterStep.skip Std.PlausibleIterStep.done
 attribute [local grind =] Std.IterStep.successor_yield Std.IterStep.successor_skip Std.IterStep.successor_done
 attribute [local grind =] Std.IterStep.mapIterator_yield
-attribute [local simp, local grind unfold] Std.Iterator.step Std.Iter.step Std.IterM.step
+attribute [local simp, local grind] Std.Iterator.step Std.Iter.step Std.IterM.step
 attribute [local simp, local grind unfold] Std.Iter.toIterM Std.IterM.toIter
 attribute [local grind =] Std.Shrink.inflate_deflate
 attribute [local grind .] Std.Iter.IsPlausibleIndirectOutput.direct
@@ -79,35 +79,40 @@ instance instIteratorLoop [Monad m] [Monad n] :
 
 variable {it : @Std.Iter (GenericIter mk size valid) α} {out : α}
 
-@[simp]
-theorem successor_isSome_iff_idx_lt_size :
+@[simp, grind .]
+theorem step_ne_skip {it'} :
+    it.step.val ≠ .skip it' := by
+  simp; grind
+
+@[local simp]
+private theorem successor_isSome_iff_idx_lt_size :
     it.step.val.successor.isSome ↔ it.internalState.idx < size := by
-  grind
+  simp; grind
 
 local grind_pattern successor_isSome_iff_idx_lt_size => it.step.val.successor
 
-@[simp, grind =]
-theorem successor_idx_eq_idx_add_one (lt : it.internalState.idx < size) :
+@[local simp, local grind =]
+private theorem successor_idx_eq_idx_add_one (lt : it.internalState.idx < size) :
     (it.step.val.successor.get (by grind) |>.internalState.idx) = it.internalState.idx + 1 := by
-  grind
+  simp; grind
 
-@[simp]
-theorem successor_eq_idx_add_one (lt : it.internalState.idx < size) :
+@[local simp]
+private theorem successor_eq_idx_add_one (lt : it.internalState.idx < size) :
     it.step.val.successor.get (by grind) = ⟨⟨it.internalState.idx + 1⟩⟩ := by
-  grind
+  simp; grind
 
 local grind_pattern successor_eq_idx_add_one => it.step.val.successor
 
-@[simp, grind =]
-theorem IsPlausibleOutput_iff :
+@[local simp, local grind =]
+private theorem IsPlausibleOutput_iff :
     it.IsPlausibleOutput out ↔
       it.internalState.idx < size ∧ out = mk it.internalState.idx := by
   simp
   intros
   exists ⟨⟨it.internalState.idx + 1⟩⟩
 
-@[simp, grind =]
-theorem IsPlausibleSuccessorOf_iff {it' : @Std.Iter (GenericIter mk size valid) α} :
+@[local simp, local grind =]
+private theorem IsPlausibleSuccessorOf_iff {it' : @Std.Iter (GenericIter mk size valid) α} :
     it'.IsPlausibleSuccessorOf it ↔
       it.internalState.idx < size ∧
       it'.internalState.idx = it.internalState.idx + 1 := by
@@ -118,8 +123,8 @@ theorem IsPlausibleSuccessorOf_iff {it' : @Std.Iter (GenericIter mk size valid) 
     exists it.step.val
     grind [Std.Iter, GenericIter]
 
-@[simp, grind =]
-theorem IsPlausibleIndirectOutput_iff :
+@[local simp, local grind =]
+private theorem IsPlausibleIndirectOutput_iff :
     it.IsPlausibleIndirectOutput out ↔
       ∃ (n : Nat) (_ : n < size) (_ : n ≥ it.internalState.idx), mk n = out := by
   constructor
@@ -146,11 +151,33 @@ instance instForIn' [Monad n] [lawful : LawfulValid mk size valid] :
     Std.IteratorLoop.finiteForIn' (fun _ _ f c => f c.run) |>.forIn' it.toIterM init
       fun out h acc => f out (by grind [lawful.hvalid]) acc
 
-@[local grind =]
+@[local simp, local grind =]
 private theorem length_eq_size_sub_idx :
     it.length = size - it.internalState.idx := by
   induction hi : size - it.internalState.idx generalizing it
-  <;> grind [Std.Iter.length_eq_match_step]
+  <;> rw [Std.Iter.length_eq_match_step]
+  <;> simp
+  <;> grind
+
+@[simp]
+theorem length_lt_yield {it' out} (eq : it.step.val = .yield it' out) :
+    it'.length < it.length := by
+  grind
+
+grind_pattern length_lt_yield => it'.length < it.length, Std.IterStep.yield it' out, it.step
+grind_pattern length_lt_yield => it'.length ≤ it.length, Std.IterStep.yield it' out, it.step
+grind_pattern length_lt_yield => it'.length > it.length, Std.IterStep.yield it' out, it.step
+grind_pattern length_lt_yield => it'.length ≥ it.length, Std.IterStep.yield it' out, it.step
+
+@[simp]
+theorem length_lt_skip {it'} (eq : it.step.val = .skip it') :
+    it'.length < it.length := by
+  grind
+
+grind_pattern length_lt_skip => it'.length < it.length, Std.IterStep.skip it', it.step
+grind_pattern length_lt_skip => it'.length ≤ it.length, Std.IterStep.skip it', it.step
+grind_pattern length_lt_skip => it'.length > it.length, Std.IterStep.skip it', it.step
+grind_pattern length_lt_skip => it'.length ≥ it.length, Std.IterStep.skip it', it.step
 
 /-
 This isn't public as the ordering of elements is an implementation detail, we may wish to
@@ -166,7 +193,7 @@ private theorem toList_eq_ofFn_mk_idx_add :
     split
     · simp; grind
     · grind
-    · grind
+    · simp_all; grind
 
 @[simp, grind =]
 private theorem mem_toList_iff_valid_of_idx_eq_zero [lawful : LawfulValid mk size valid] {idx : α}
@@ -180,6 +207,14 @@ private theorem mem_toList_iff_valid_of_idx_eq_zero [lawful : LawfulValid mk siz
     rcases h with ⟨n, _⟩
     exists ⟨n, by grind⟩
     grind
+
+private theorem yield_var_eq_internalState (h : it.step.val = .yield it' var) :
+    var = mk it.internalState.idx := by
+  grind
+
+private theorem yield_it_eq_inc (h : it.step.val = .yield it' var) :
+    it'.internalState.idx = it.internalState.idx + 1 := by
+  grind
 
 end GenericIter
 
@@ -271,14 +306,67 @@ theorem mem_iter_toList_iff_valid {var : Var} :
     var ∈ aig.iter.toList ↔ var.validIn aig := by
   grind [iter]
 
-theorem iter_toList_ne_of_ne :
-    ∀ {i j : Nat} (hi : i < aig.size) (hj : j < aig.size) (_ : i ≠ j),
-      aig.iter.toList[i]'(by simpa) ≠ aig.iter.toList[j]'(by simpa) := by
+@[simp, grind =]
+theorem iter_toList_eq :
+    aig.iter.toList = .ofFn (fun (n : Fin aig.size) => .ofIdx n) := by
   simp
+  rw [length_iter_eq_size]
+  grind [iter]
 
-theorem iter_toList_lt_of_lt :
-    ∀ {i j : Nat} (hi : i < aig.size) (hj : j < aig.size) (_ : i < j),
-      aig.iter.toList[i]'(by simpa) < aig.iter.toList[j]'(by simpa) := by
-  simp [Var.lt_idx]
+/--
+Convenience function to access the current state of `Aig.iter`, which is guaranteed to
+be the next returned value if the iterator is still valid.
+-/
+@[always_inline]
+def _root_.Std.Iter.var (it : @Std.Iter (VarIterator aig) Var) : Var :=
+  .ofIdx it.internalState.idx
+
+variable {it it' : @Std.Iter (VarIterator aig) Var}
+
+@[simp]
+theorem length_eq_size_sub_var_idx :
+    it.length = aig.size - it.var.idx := by
+  simp [Std.Iter.var, GenericIter.length_eq_size_sub_idx]
+
+@[simp, grind =]
+theorem iter_var_eq_zero :
+    aig.iter.var = .ofIdx 0 := by
+  simp [iter, Std.Iter.var]
+
+@[simp, grind .]
+theorem iter_yield_eq_var (h : it.step.val = .yield it' var) :
+    var = it.var := by
+  grind only [Std.Iter.var, GenericIter.yield_var_eq_internalState]
+
+@[simp]
+theorem iter_yield_var_eq_var_add_one (h : it.step.val = .yield it' var) :
+    it'.var = it.var + 1 := by
+  simp [Std.Iter.var, Var.ext_idx]
+  grind only [GenericIter.yield_it_eq_inc]
+
+grind_pattern iter_yield_var_eq_var_add_one => Std.IterStep.yield it' var, it.var
+
+/--
+Forward fold across all valid variables, accumulating a map from each variable to some element as
+well as a custom state. This is useful for forward analyses.
+-/
+@[inline]
+def varFoldMap {α σ : Type} (aig : Aig) (init : σ)
+    (step : σ -> (var : Var) -> ((var' : Var) -> var' < var -> α) -> σ × α) : σ :=
+  go init aig.iter
+where
+  go (state : σ) (iter : Std.Iter Var) (map : Array α := #[])
+      (h : iter.var.idx = map.size := by grind) : σ :=
+    match h : iter.step.val with
+    | .yield it var =>
+      let mapF (var' : Var) (h : var' < var) :=
+        map[var'.idx]'(by grind)
+      let (state, val) := step state var mapF
+      let map := map.push val
+      go state it map
+    | .done => state
+    | .skip it => go state it map
+  termination_by iter.length
+  decreasing_by all_goals grind
 
 end var
